test: cleanup

tests/lean/run/linearByRefl2.lean
@@ -1,5 +1,21 @@
 abbrev Var := Nat
 
+structure Context where
+  vars : List Nat
+
+private def List.getIdx : List α → Nat → α → α
+  | [],    i,   u => u
+  | a::as, 0,   u => a
+  | a::as, i+1, u => getIdx as i u
+
+/--
+  When encoding polynomials. We use `fixedVar` for encoding numerals.
+  The denotation of `fixedVar` is always `1`. -/
+def fixedVar := 100000000 -- Any big number should work here
+
+def Var.denote (ctx : Context) (v : Var) : Nat :=
+  if v = fixedVar then 1 else ctx.vars.getIdx v 0
+
 inductive Expr where
   | num  (v : Nat)
   | var  (i : Var)
@@ -8,30 +24,12 @@ inductive Expr where
   | mulR (a : Expr) (k : Nat)
   deriving Inhabited, Repr
 
-/--
-  When encoding polynomials. We use `fixedVar` for encoding numerals.
-  The denotation of `fixedVar` is always `1`. -/
-def fixedVar := 100000000 -- Any big number should work here
-
-structure Context where
-  vars : List Nat
-
-private def List.getIdx : List α → Var → α → α
-  | [],    i,   u => u
-  | a::as, 0,   u => a
-  | a::as, i+1, u => getIdx as i u
-
-def Var.denote (ctx : Context) (v : Var) : Nat :=
-  if v = fixedVar then 1 else ctx.vars.getIdx v 0
-
 def Expr.denote (ctx : Context) : Expr → Nat
   | Expr.add a b  => Nat.add (denote ctx a) (denote ctx b)
   | Expr.num k    => k
   | Expr.var v    => v.denote ctx
   | Expr.mulL k e => k * denote ctx e
   | Expr.mulR e k => denote ctx e * k
-
-attribute [local simp] Nat.add_comm Nat.add_assoc Nat.add_left_comm Nat.right_distrib Nat.left_distrib Nat.mul_assoc Nat.mul_comm
 
 abbrev Poly := List (Nat × Var)
 
@@ -45,43 +43,12 @@ def Poly.insertSorted (k : Nat) (v : Var) (p : Poly) : Poly :=
   | [] => [(k, v)]
   | (k', v') :: p => if v < v' then (k, v) :: (k', v') :: p else (k', v') :: insertSorted k v p
 
-@[simp] theorem Poly.denote_insertSorted (ctx : Context) (k : Nat) (v : Var) (p : Poly) : (p.insertSorted k v).denote ctx = p.denote ctx + k * v.denote ctx := by
-  match p with
-  | [] => simp [insertSorted, denote]
-  | (k', v') :: p => by_cases h : v < v' <;> simp [h, insertSorted, denote, denote_insertSorted]
-
 def Poly.sort (p : Poly) : Poly :=
   let rec go (p : Poly) (r : Poly) : Poly :=
     match p with
     | [] => r
     | (k, v) :: p => go p (r.insertSorted k v)
   go p []
-
-@[simp] theorem Poly.denote_sort_go (ctx : Context) (p : Poly) (r : Poly) : (sort.go p r).denote ctx = p.denote ctx + r.denote ctx := by
-  match p with
-  | [] => simp [sort.go, denote]
-  | (k, v):: p => simp [sort.go, denote, denote_sort_go]
-
-@[simp] theorem Poly.denote_sort (ctx : Context) (m : Poly) : m.sort.denote ctx = m.denote ctx := by
-  simp [sort, denote]
-
-@[simp] theorem Poly.denote_append (ctx : Context) (p q : Poly) : (p ++ q).denote ctx = p.denote ctx + q.denote ctx := by
-  match p with
-  | []  => simp [denote]
-  | (k, v) :: p => simp [denote, denote_append]
-
-@[simp] theorem Poly.denote_cons (ctx : Context) (k : Nat) (v : Var) (p : Poly) : denote ctx ((k, v) :: p) = k * v.denote ctx + p.denote ctx := by
-  match p with
-  | []     => simp [denote]
-  | _ :: m => simp [denote, denote_cons]
-
-@[simp] theorem Poly.denote_reverseAux (ctx : Context) (p q : Poly) : denote ctx (List.reverseAux p q) = denote ctx (p ++ q) := by
-  match p with
-  | [] => simp [denote, List.reverseAux]
-  | (k, v) :: p => simp [denote, List.reverseAux, denote_reverseAux]
-
-@[simp] theorem Poly.denote_reverse (ctx : Context) (p : Poly) : denote ctx (List.reverse p) = denote ctx p := by
-  simp [List.reverse]
 
 def Poly.fuse (p : Poly) : Poly :=
   match p with
@@ -90,16 +57,6 @@ def Poly.fuse (p : Poly) : Poly :=
     match fuse p with
     | [] => [(k, v)]
     | (k', v') :: p' => if v = v' then (k+k', v)::p' else (k, v) :: (k', v') :: p'
-
-@[simp] theorem Poly.denote_fuse (ctx : Context) (p : Poly) : p.fuse.denote ctx = p.denote ctx := by
-  match p with
-  | [] => rfl
-  | (k, v) :: p =>
-    have ih := denote_fuse ctx p
-    simp [fuse, denote]
-    split
-    case _ h => simp [denote, ← ih, h]
-    case _ k' v' p' h => by_cases he : v = v' <;> simp [he, denote, ← ih, h]
 
 def Poly.mul (k : Nat) (p : Poly) : Poly :=
   if k = 0 then
@@ -110,15 +67,6 @@ where
   go : Poly → Poly
   | [] => []
   | (k', v) :: p => (k*k', v) :: go p
-
-@[simp] theorem Poly.denote_mul (ctx : Context) (k : Nat) (p : Poly) : (p.mul k).denote ctx = k * p.denote ctx := by
-  simp [mul]
-  by_cases h : k = 0
-  . simp [denote, h]
-  . simp [denote, h]
-    induction p with
-    | nil  => simp [mul.go, denote]
-    | cons kv m ih => cases kv with | _ k' v => simp [mul.go, denote, ih]
 
 def Poly.cancelAux (fuel : Nat) (m₁ m₂ r₁ r₂ : Poly) : Poly × Poly :=
   match fuel with
@@ -139,24 +87,130 @@ def Poly.cancelAux (fuel : Nat) (m₁ m₂ r₁ r₂ : Poly) : Poly × Poly :=
       else
         cancelAux fuel m₁ m₂ r₁ r₂
 
+def Poly.cancel (m₁ m₂ : Poly) : Poly × Poly :=
+  cancelAux (m₁.length + m₂.length) m₁ m₂ [] []
+
 def Poly.denote_eq (ctx : Context) (mp : Poly × Poly) : Prop := mp.1.denote ctx = mp.2.denote ctx
+
+def Poly.denote_le (ctx : Context) (mp : Poly × Poly) : Prop := mp.1.denote ctx ≤ mp.2.denote ctx
+
+def Expr.toPoly : Expr → Poly
+  | Expr.num k    => if k = 0 then [] else [ (k, fixedVar) ]
+  | Expr.var i    => [(1, i)]
+  | Expr.add a b  => a.toPoly ++ b.toPoly
+  | Expr.mulL k a => a.toPoly.mul k
+  | Expr.mulR a k => a.toPoly.mul k
+
+def Expr.toNormPoly (e : Expr) : Poly :=
+  e.toPoly.sort.fuse
+
+def Expr.inc (e : Expr) : Expr :=
+   Expr.add e (Expr.num 1)
+
+structure ExprLe where
+  lhs : Expr
+  rhs : Expr
+  deriving Repr
+
+def ExprLe.denote (ctx : Context) (c : ExprLe) := c.lhs.denote ctx ≤ c.rhs.denote ctx
+
+def ExprLe.add (c d : ExprLe) : ExprLe :=
+  { lhs := Expr.add c.lhs d.lhs, rhs := Expr.add c.rhs d.rhs }
+
+def ExprLe.toNormPoly (c : ExprLe) : Poly × Poly :=
+  Poly.cancel c.lhs.toNormPoly c.rhs.toNormPoly
+
+def ExprLe.toPoly (c : ExprLe) : Poly × Poly :=
+  (c.lhs.toPoly, c.rhs.toPoly)
+
+attribute [local simp] Nat.add_comm Nat.add_assoc Nat.add_left_comm Nat.right_distrib Nat.left_distrib Nat.mul_assoc Nat.mul_comm
+
+attribute [local simp] Poly.denote Expr.denote Poly.insertSorted Poly.sort Poly.sort.go Poly.fuse Poly.cancelAux Poly.cancel
+attribute [local simp] Poly.mul Poly.mul.go
+
+theorem Poly.denote_insertSorted (ctx : Context) (k : Nat) (v : Var) (p : Poly) : (p.insertSorted k v).denote ctx = p.denote ctx + k * v.denote ctx := by
+  match p with
+  | [] => simp
+  | (k', v') :: p => by_cases h : v < v' <;> simp [h, denote_insertSorted]
+
+attribute [local simp] Poly.denote_insertSorted
+
+theorem Poly.denote_sort_go (ctx : Context) (p : Poly) (r : Poly) : (sort.go p r).denote ctx = p.denote ctx + r.denote ctx := by
+  match p with
+  | [] => simp
+  | (k, v):: p => simp [denote_sort_go]
+
+attribute [local simp] Poly.denote_sort_go
+
+theorem Poly.denote_sort (ctx : Context) (m : Poly) : m.sort.denote ctx = m.denote ctx := by
+  simp
+
+attribute [local simp] Poly.denote_sort
+
+theorem Poly.denote_append (ctx : Context) (p q : Poly) : (p ++ q).denote ctx = p.denote ctx + q.denote ctx := by
+  match p with
+  | []  => simp
+  | (k, v) :: p => simp [denote_append]
+
+attribute [local simp] Poly.denote_append
+
+theorem Poly.denote_cons (ctx : Context) (k : Nat) (v : Var) (p : Poly) : denote ctx ((k, v) :: p) = k * v.denote ctx + p.denote ctx := by
+  match p with
+  | []     => simp
+  | _ :: m => simp [denote_cons]
+
+attribute [local simp] Poly.denote_cons
+
+theorem Poly.denote_reverseAux (ctx : Context) (p q : Poly) : denote ctx (List.reverseAux p q) = denote ctx (p ++ q) := by
+  match p with
+  | [] => simp [List.reverseAux]
+  | (k, v) :: p => simp [List.reverseAux, denote_reverseAux]
+
+attribute [local simp] Poly.denote_reverseAux
+
+theorem Poly.denote_reverse (ctx : Context) (p : Poly) : denote ctx (List.reverse p) = denote ctx p := by
+  simp [List.reverse]
+
+attribute [local simp] Poly.denote_reverse
+
+theorem Poly.denote_fuse (ctx : Context) (p : Poly) : p.fuse.denote ctx = p.denote ctx := by
+  match p with
+  | [] => rfl
+  | (k, v) :: p =>
+    have ih := denote_fuse ctx p
+    simp
+    split
+    case _ h => simp [← ih, h]
+    case _ k' v' p' h => by_cases he : v = v' <;> simp [he, ← ih, h]
+
+attribute [local simp] Poly.denote_fuse
+
+theorem Poly.denote_mul (ctx : Context) (k : Nat) (p : Poly) : (p.mul k).denote ctx = k * p.denote ctx := by
+  simp
+  by_cases h : k = 0 <;> simp [h]
+  simp [h]
+  induction p with
+  | nil  => simp
+  | cons kv m ih => cases kv with | _ k' v => simp [ih]
+
+attribute [local simp] Poly.denote_mul
 
 theorem Poly.denote_eq_cancelAux (ctx : Context) (fuel : Nat) (m₁ m₂ r₁ r₂ : Poly)
     (h : denote_eq ctx (r₁.reverse ++ m₁, r₂.reverse ++ m₂)) : denote_eq ctx (cancelAux fuel m₁ m₂ r₁ r₂) := by
   induction fuel generalizing m₁ m₂ r₁ r₂ with
   | zero => assumption
   | succ fuel ih =>
-    simp [cancelAux]
+    simp
     split <;> simp at h <;> try assumption
     rename_i k₁ v₁ m₁ k₂ v₂ m₂
     by_cases hltv : v₁ < v₂ <;> simp [hltv]
-    . apply ih; simp [denote_eq, denote] at h |-; assumption
+    . apply ih; simp [denote_eq] at h |-; assumption
     . by_cases hgtv : v₁ > v₂ <;> simp [hgtv]
-      . apply ih; simp [denote_eq, denote] at h |-; assumption
+      . apply ih; simp [denote_eq] at h |-; assumption
       . have heqv : v₁ = v₂ := Nat.le_antisymm (Nat.ge_of_not_lt hgtv) (Nat.ge_of_not_lt hltv); subst heqv
         by_cases hltk : k₁ < k₂ <;> simp [hltk]
         . apply ih
-          simp [denote_eq, denote] at h |-
+          simp [denote_eq] at h |-
           have haux : k₁ * Var.denote ctx v₁ ≤ k₂ * Var.denote ctx v₁ := Nat.mul_le_mul_right _ (Nat.le_of_lt hltk)
           rw [Nat.mul_sub_right_distrib, ← Nat.add_assoc, ← Nat.add_sub_assoc haux]
           apply Eq.symm
@@ -164,14 +218,14 @@ theorem Poly.denote_eq_cancelAux (ctx : Context) (fuel : Nat) (m₁ m₂ r₁ r�
           simp [h]
         . by_cases hgtk : k₁ > k₂ <;> simp [hgtk]
           . apply ih
-            simp [denote_eq, denote] at h |-
+            simp [denote_eq] at h |-
             have haux : k₂ * Var.denote ctx v₁ ≤ k₁ * Var.denote ctx v₁ := Nat.mul_le_mul_right _ (Nat.le_of_lt hgtk)
             rw [Nat.mul_sub_right_distrib, ← Nat.add_assoc, ← Nat.add_sub_assoc haux]
             apply Nat.sub_eq_of_eq_add
             simp [h]
           . have heqk : k₁ = k₂ := Nat.le_antisymm (Nat.ge_of_not_lt hgtk) (Nat.ge_of_not_lt hltk); subst heqk
             apply ih
-            simp [denote_eq, denote] at h |-
+            simp [denote_eq] at h |-
             rw [← Nat.add_assoc, ← Nat.add_assoc] at h
             exact Nat.add_right_cancel h
 
@@ -180,40 +234,37 @@ theorem Poly.of_denote_eq_cancelAux (ctx : Context) (fuel : Nat) (m₁ m₂ r₁
   induction fuel generalizing m₁ m₂ r₁ r₂ with
   | zero => assumption
   | succ fuel ih =>
-    simp [cancelAux] at h
+    simp at h
     split at h <;> simp <;> try assumption
     rename_i k₁ v₁ m₁ k₂ v₂ m₂
     by_cases hltv : v₁ < v₂ <;> simp [hltv] at h
-    . have ih := ih (h := h); simp [denote_eq, denote] at ih ⊢; assumption
+    . have ih := ih (h := h); simp [denote_eq] at ih ⊢; assumption
     . by_cases hgtv : v₁ > v₂ <;> simp [hgtv] at h
-      . have ih := ih (h := h); simp [denote_eq, denote] at ih ⊢; assumption
+      . have ih := ih (h := h); simp [denote_eq] at ih ⊢; assumption
       . have heqv : v₁ = v₂ := Nat.le_antisymm (Nat.ge_of_not_lt hgtv) (Nat.ge_of_not_lt hltv); subst heqv
         by_cases hltk : k₁ < k₂ <;> simp [hltk] at h
-        . have ih := ih (h := h); simp [denote_eq, denote] at ih ⊢
+        . have ih := ih (h := h); simp [denote_eq] at ih ⊢
           have haux : k₁ * Var.denote ctx v₁ ≤ k₂ * Var.denote ctx v₁ := Nat.mul_le_mul_right _ (Nat.le_of_lt hltk)
           rw [Nat.mul_sub_right_distrib, ← Nat.add_assoc, ← Nat.add_sub_assoc haux] at ih
           have ih := Nat.eq_add_of_sub_eq (Nat.le_trans haux (Nat.le_add_left ..)) ih.symm
           simp at ih
           rw [ih]
         . by_cases hgtk : k₁ > k₂ <;> simp [hgtk] at h
-          . have ih := ih (h := h); simp [denote_eq, denote] at ih ⊢
+          . have ih := ih (h := h); simp [denote_eq] at ih ⊢
             have haux : k₂ * Var.denote ctx v₁ ≤ k₁ * Var.denote ctx v₁ := Nat.mul_le_mul_right _ (Nat.le_of_lt hgtk)
             rw [Nat.mul_sub_right_distrib, ← Nat.add_assoc, ← Nat.add_sub_assoc haux] at ih
             have ih := Nat.eq_add_of_sub_eq (Nat.le_trans haux (Nat.le_add_left ..)) ih
             simp at ih
             rw [ih]
           . have heqk : k₁ = k₂ := Nat.le_antisymm (Nat.ge_of_not_lt hgtk) (Nat.ge_of_not_lt hltk); subst heqk
-            have ih := ih (h := h); simp [denote_eq, denote] at ih ⊢
+            have ih := ih (h := h); simp [denote_eq] at ih ⊢
             rw [← Nat.add_assoc, ih, Nat.add_assoc]
 
-def Poly.cancel (m₁ m₂ : Poly) : Poly × Poly :=
-  cancelAux (m₁.length + m₂.length) m₁ m₂ [] []
-
 theorem Poly.denote_eq_cancel {ctx : Context} {m₁ m₂ : Poly} (h : denote_eq ctx (m₁, m₂)) : denote_eq ctx (cancel m₁ m₂) := by
-  simp [cancel]; apply denote_eq_cancelAux; simp [h]
+  simp; apply denote_eq_cancelAux; simp [h]
 
 theorem Poly.of_denote_eq_cancel {ctx : Context} {m₁ m₂ : Poly} (h : denote_eq ctx (cancel m₁ m₂)) : denote_eq ctx (m₁, m₂) := by
-  simp [cancel] at h
+  simp at h
   have := Poly.of_denote_eq_cancelAux (h := h)
   simp at this
   assumption
@@ -221,38 +272,36 @@ theorem Poly.of_denote_eq_cancel {ctx : Context} {m₁ m₂ : Poly} (h : denote_
 theorem Poly.denote_eq_cancel_eq (ctx : Context) (m₁ m₂ : Poly) : denote_eq ctx (cancel m₁ m₂) = denote_eq ctx (m₁, m₂) :=
   propext <| Iff.intro (fun h => of_denote_eq_cancel h) (fun h => denote_eq_cancel h)
 
-def Poly.denote_le (ctx : Context) (mp : Poly × Poly) : Prop := mp.1.denote ctx ≤ mp.2.denote ctx
-
 theorem Poly.denote_le_cancelAux (ctx : Context) (fuel : Nat) (m₁ m₂ r₁ r₂ : Poly)
     (h : denote_le ctx (r₁.reverse ++ m₁, r₂.reverse ++ m₂)) : denote_le ctx (cancelAux fuel m₁ m₂ r₁ r₂) := by
   induction fuel generalizing m₁ m₂ r₁ r₂ with
   | zero => assumption
   | succ fuel ih =>
-    simp [cancelAux]
+    simp
     split <;> simp at h <;> try assumption
     rename_i k₁ v₁ m₁ k₂ v₂ m₂
     by_cases hltv : v₁ < v₂ <;> simp [hltv]
-    . apply ih; simp [denote_le, denote] at h |-; assumption
+    . apply ih; simp [denote_le] at h |-; assumption
     . by_cases hgtv : v₁ > v₂ <;> simp [hgtv]
-      . apply ih; simp [denote_le, denote] at h |-; assumption
+      . apply ih; simp [denote_le] at h |-; assumption
       . have heqv : v₁ = v₂ := Nat.le_antisymm (Nat.ge_of_not_lt hgtv) (Nat.ge_of_not_lt hltv); subst heqv
         by_cases hltk : k₁ < k₂ <;> simp [hltk]
         . apply ih
-          simp [denote_le, denote] at h |-
+          simp [denote_le] at h |-
           have haux : k₁ * Var.denote ctx v₁ ≤ k₂ * Var.denote ctx v₁ := Nat.mul_le_mul_right _ (Nat.le_of_lt hltk)
           rw [Nat.mul_sub_right_distrib, ← Nat.add_assoc, ← Nat.add_sub_assoc haux]
           apply Nat.le_sub_of_add_le
           simp [h]
         . by_cases hgtk : k₁ > k₂ <;> simp [hgtk]
           . apply ih
-            simp [denote_le, denote] at h |-
+            simp [denote_le] at h |-
             have haux : k₂ * Var.denote ctx v₁ ≤ k₁ * Var.denote ctx v₁ := Nat.mul_le_mul_right _ (Nat.le_of_lt hgtk)
             rw [Nat.mul_sub_right_distrib, ← Nat.add_assoc, ← Nat.add_sub_assoc haux]
             apply Nat.sub_le_of_le_add (Nat.le_trans haux (Nat.le_add_left ..))
             simp [h]
           . have heqk : k₁ = k₂ := Nat.le_antisymm (Nat.ge_of_not_lt hgtk) (Nat.ge_of_not_lt hltk); subst heqk
             apply ih
-            simp [denote_le, denote] at h |-
+            simp [denote_le] at h |-
             rw [← Nat.add_assoc, ← Nat.add_assoc] at h
             apply Nat.le_of_add_le_add_right h
     done
@@ -262,39 +311,39 @@ theorem Poly.of_denote_le_cancelAux (ctx : Context) (fuel : Nat) (m₁ m₂ r₁
   induction fuel generalizing m₁ m₂ r₁ r₂ with
   | zero => assumption
   | succ fuel ih =>
-    simp [cancelAux] at h
+    simp at h
     split at h <;> simp <;> try assumption
     rename_i k₁ v₁ m₁ k₂ v₂ m₂
     by_cases hltv : v₁ < v₂ <;> simp [hltv] at h
-    . have ih := ih (h := h); simp [denote_le, denote] at ih ⊢; assumption
+    . have ih := ih (h := h); simp [denote_le] at ih ⊢; assumption
     . by_cases hgtv : v₁ > v₂ <;> simp [hgtv] at h
-      . have ih := ih (h := h); simp [denote_le, denote] at ih ⊢; assumption
+      . have ih := ih (h := h); simp [denote_le] at ih ⊢; assumption
       . have heqv : v₁ = v₂ := Nat.le_antisymm (Nat.ge_of_not_lt hgtv) (Nat.ge_of_not_lt hltv); subst heqv
         by_cases hltk : k₁ < k₂ <;> simp [hltk] at h
-        . have ih := ih (h := h); simp [denote_le, denote] at ih ⊢
+        . have ih := ih (h := h); simp [denote_le] at ih ⊢
           have haux : k₁ * Var.denote ctx v₁ ≤ k₂ * Var.denote ctx v₁ := Nat.mul_le_mul_right _ (Nat.le_of_lt hltk)
           rw [Nat.mul_sub_right_distrib, ← Nat.add_assoc, ← Nat.add_sub_assoc haux] at ih
           have := Nat.add_le_of_le_sub (Nat.le_trans haux (Nat.le_add_left ..)) ih
           simp at this
           exact this
         . by_cases hgtk : k₁ > k₂ <;> simp [hgtk] at h
-          . have ih := ih (h := h); simp [denote_le, denote] at ih ⊢
+          . have ih := ih (h := h); simp [denote_le] at ih ⊢
             have haux : k₂ * Var.denote ctx v₁ ≤ k₁ * Var.denote ctx v₁ := Nat.mul_le_mul_right _ (Nat.le_of_lt hgtk)
             rw [Nat.mul_sub_right_distrib, ← Nat.add_assoc, ← Nat.add_sub_assoc haux] at ih
             have := Nat.le_add_of_sub_le (Nat.le_trans haux (Nat.le_add_left ..)) ih
             simp at this
             exact this
           . have heqk : k₁ = k₂ := Nat.le_antisymm (Nat.ge_of_not_lt hgtk) (Nat.ge_of_not_lt hltk); subst heqk
-            have ih := ih (h := h); simp [denote_le, denote] at ih ⊢
+            have ih := ih (h := h); simp [denote_le] at ih ⊢
             have := Nat.add_le_add_right ih (k₁ * Var.denote ctx v₁)
             simp at this
             exact this
 
 theorem Poly.denote_le_cancel {ctx : Context} {m₁ m₂ : Poly} (h : denote_le ctx (m₁, m₂)) : denote_le ctx (cancel m₁ m₂) := by
-  simp [cancel]; apply denote_le_cancelAux; simp [h]
+  simp; apply denote_le_cancelAux; simp [h]
 
 theorem Poly.of_denote_le_cancel {ctx : Context} {m₁ m₂ : Poly} (h : denote_le ctx (cancel m₁ m₂)) : denote_le ctx (m₁, m₂) := by
-  simp [cancel] at h
+  simp at h
   have := Poly.of_denote_le_cancelAux (h := h)
   simp at this
   assumption
@@ -302,23 +351,13 @@ theorem Poly.of_denote_le_cancel {ctx : Context} {m₁ m₂ : Poly} (h : denote_
 theorem Poly.denote_le_cancel_eq (ctx : Context) (m₁ m₂ : Poly) : denote_le ctx (cancel m₁ m₂) = denote_le ctx (m₁, m₂) :=
   propext <| Iff.intro (fun h => of_denote_le_cancel h) (fun h => denote_le_cancel h)
 
-def Expr.toPoly : Expr → Poly
-  | Expr.num k    => if k = 0 then [] else [ (k, fixedVar) ]
-  | Expr.var i    => [(1, i)]
-  | Expr.add a b  => a.toPoly ++ b.toPoly
-  | Expr.mulL k a => a.toPoly.mul k
-  | Expr.mulR a k => a.toPoly.mul k
-
 @[simp] theorem Expr.denote_toPoly (ctx : Context) (e : Expr) : e.toPoly.denote ctx = e.denote ctx := by
   induction e with
-  | num k => by_cases h : k = 0 <;> simp [toPoly, h, Poly.denote, Var.denote, denote]
-  | var i => simp [denote, toPoly, Poly.denote, Poly.denote]
-  | add a b iha ihb => simp [denote, toPoly, iha, ihb]; done
-  | mulL k a ih => simp [denote, toPoly, ih]; done
-  | mulR k a ih => simp [denote, toPoly, ih]; done
-
-def Expr.toNormPoly (e : Expr) : Poly :=
-  e.toPoly.sort.fuse
+  | num k => by_cases h : k = 0 <;> simp [toPoly, h, Var.denote]
+  | var i => simp [toPoly]
+  | add a b iha ihb => simp [toPoly, iha, ihb]
+  | mulL k a ih => simp [toPoly, ih, -Poly.mul]
+  | mulR k a ih => simp [toPoly, ih, -Poly.mul]
 
 theorem Expr.eq_of_toNormPoly (ctx : Context) (a b : Expr) (h : a.toNormPoly = b.toNormPoly) : a.denote ctx = b.denote ctx := by
   simp [toNormPoly] at h
@@ -338,29 +377,11 @@ theorem Expr.of_cancel_le (ctx : Context) (a b c d : Expr) (h : Poly.cancel a.to
   simp [toNormPoly, Poly.denote_le] at this
   exact this.symm
 
-def Expr.inc (e : Expr) : Expr :=
-   Expr.add e (Expr.num 1)
-
 theorem Expr.of_cancel_lt (ctx : Context) (a b c d : Expr) (h : Poly.cancel a.inc.toNormPoly b.toNormPoly = (c.inc.toPoly, d.toPoly)) : (a.denote ctx < b.denote ctx) = (c.denote ctx < d.denote ctx) :=
   of_cancel_le ctx a.inc b c.inc d h
 
-structure ExprLe where
-  lhs : Expr
-  rhs : Expr
-  deriving Repr
-
-def ExprLe.denote (ctx : Context) (c : ExprLe) := c.lhs.denote ctx ≤ c.rhs.denote ctx
-
-def ExprLe.add (c d : ExprLe) : ExprLe :=
-  { lhs := Expr.add c.lhs d.lhs, rhs := Expr.add c.rhs d.rhs }
-
-def ExprLe.toNormPoly (c : ExprLe) : Poly × Poly :=
-  Poly.cancel c.lhs.toNormPoly c.rhs.toNormPoly
-
-def ExprLe.toPoly (c : ExprLe) : Poly × Poly :=
-  (c.lhs.toPoly, c.rhs.toPoly)
-
-theorem ExprLe.combine (ctx : Context) (c d e : ExprLe) (h₁ : c.denote ctx) (h₂ : d.denote ctx) (h₃ : e.toPoly = (c.add d).toNormPoly) : e.denote ctx := by
+theorem ExprLe.combine (ctx : Context) (c d e : ExprLe) (h₃ : e.toPoly = (c.add d).toNormPoly) : c.denote ctx → d.denote ctx → e.denote ctx := by
+  intro h₁ h₂
   match c, d, e with
   | { lhs := cLhs, rhs := cRhs }, { lhs := dLhs, rhs := dRhs }, { lhs := eLhs, rhs := eRhs } =>
     simp [add, denote, Expr.denote, toPoly, toNormPoly] at h₁ h₂ h₃ |-
@@ -397,11 +418,9 @@ example (x₁ x₂ x₃ : Nat) : ((x₁ + x₂) + (x₂ + x₃) < x₃ + x₂) =
     (Expr.num 0)
     rfl
 
-example (x₁ x₂) (h₁ : x₁ + 2 ≤ 3*x₂) (h₂ : 4*x₂ ≤ 3 + x₁) : x₂ ≤ 1 :=
+example (x₁ x₂ : Nat) : x₁ + 2 ≤ 3*x₂ → 4*x₂ ≤ 3 + x₁ → x₂ ≤ 1 :=
   ExprLe.combine { vars := [x₁, x₂] }
     { lhs := Expr.add (Expr.var 0) (Expr.num 2), rhs := Expr.mulL 3 (Expr.var 1) }
     { lhs := Expr.mulL 4 (Expr.var 1), rhs := Expr.add (Expr.num 3) (Expr.var 0) }
     { lhs := Expr.var 1, rhs := Expr.num 1 }
-    h₁
-    h₂
     rfl
